compiler/bootstrap/translation/compiler64_preludeProgScript.sml
@@ -1,0 +1,155 @@
+open preamble;
+open terminationTheory
+open ml_translatorLib ml_translatorTheory;
+open std_preludeTheory;
+
+val _ = new_theory "compiler64_preludeProg"
+
+(* temporary *)
+val _ = translation_extends "std_prelude";
+
+val RW = REWRITE_RULE
+val RW1 = ONCE_REWRITE_RULE
+fun list_dest f tm =
+  let val (x,y) = f tm in list_dest f x @ list_dest f y end
+  handle HOL_ERR _ => [tm];
+val dest_fun_type = dom_rng
+val mk_fun_type = curry op -->;
+fun list_mk_fun_type [ty] = ty
+  | list_mk_fun_type (ty1::tys) =
+      mk_fun_type ty1 (list_mk_fun_type tys)
+  | list_mk_fun_type _ = fail()
+
+val _ = add_preferred_thy "-";
+val _ = add_preferred_thy "termination";
+
+val NOT_NIL_AND_LEMMA = prove(
+  ``(b <> [] /\ x) = if b = [] then F else x``,
+  Cases_on `b` THEN FULL_SIMP_TAC std_ss []);
+
+val extra_preprocessing = ref [MEMBER_INTRO,MAP];
+
+val matches = ref ([]: term list);
+
+fun def_of_const tm = let
+  val res = dest_thy_const tm handle HOL_ERR _ =>
+              failwith ("Unable to translate: " ^ term_to_string tm)
+  val name = (#Name res)
+  fun def_from_thy thy name =
+    DB.fetch thy (name ^ "_def") handle HOL_ERR _ =>
+    DB.fetch thy (name ^ "_DEF") handle HOL_ERR _ =>
+    DB.fetch thy (name ^ "_thm") handle HOL_ERR _ =>
+    DB.fetch thy name
+  val def = def_from_thy "termination" name handle HOL_ERR _ =>
+            def_from_thy (#Thy res) name handle HOL_ERR _ =>
+            failwith ("Unable to find definition of " ^ name)
+
+  val insts = if exists (fn term => can (find_term (can (match_term term))) (concl def)) (!matches) then [alpha |-> ``:64``] else []
+
+  val def = def |> INST_TYPE insts
+                |> CONV_RULE (DEPTH_CONV BETA_CONV)
+                (* TODO: This ss messes up defs containing if-then-else
+                with constant branches
+                |> SIMP_RULE bool_ss [IN_INSERT,NOT_IN_EMPTY]*)
+                |> REWRITE_RULE [NOT_NIL_AND_LEMMA]
+  in def end
+
+val _ = (find_def_for_const := def_of_const);
+
+val _ = use_long_names:=true;
+
+val spec64 = INST_TYPE[alpha|->``:64``]
+
+val conv64 = GEN_ALL o CONV_RULE (wordsLib.WORD_CONV) o spec64 o SPEC_ALL
+
+val conv64_RHS = GEN_ALL o CONV_RULE (RHS_CONV wordsLib.WORD_CONV) o spec64 o SPEC_ALL
+
+(* Attempts at translating bvp_to_word things *)
+open data_to_wordTheory
+
+val we_simp = SIMP_RULE std_ss [word_extract_w2w_mask,w2w_id]
+
+val wcomp_simp = SIMP_RULE std_ss [word_2comp_def]
+
+val _ = translate adjust_set_def
+
+val _ = translate (make_header_def |> SIMP_RULE std_ss [word_lsl_n2w]|> conv64_RHS)
+
+val shift_left_def = Define`
+  shift_left (a : 'a word) n =
+  if n = 0 then a
+  else if (a = 0w) \/ n > dimindex(:'a) then 0w
+  else if n > 32 then shift_left (a << 32) (n - 32)
+  else if n > 16 then shift_left (a << 16) (n - 16)
+  else if n > 8 then shift_left (a << 8) (n - 8)
+  else shift_left (a << 1) (n - 1)`
+
+val shift_left_rwt = Q.prove(
+  `!a n. a << n = shift_left a n`,
+  completeInduct_on `n`
+  \\ rw [Once shift_left_def]
+  \\ qpat_assum `!n. P` (assume_tac o GSYM)
+  \\ fs [])
+
+val shift_right_def = Define`
+  shift_right (a : 'a word) n =
+  if n = 0 then a
+  else if (a = 0w) \/ n > dimindex(:'a) then 0w
+  else if n > 32 then shift_right (a >>> 32) (n - 32)
+  else if n > 16 then shift_right (a >>> 16) (n - 16)
+  else if n > 8 then shift_right (a >>> 8) (n - 8)
+  else shift_right (a >>> 1) (n - 1)`
+
+val shift_right_rwt = Q.prove(
+  `!a n. a >>> n = shift_right a n`,
+  completeInduct_on `n`
+  \\ rw [Once shift_right_def]
+  \\ qpat_assum `!n. P` (assume_tac o GSYM)
+  \\ fs [])
+
+val _ = translate (shift_left_def |> conv64)
+val _ = translate (shift_right_def |> spec64 |> CONV_RULE fcpLib.INDEX_CONV)
+
+val _ = translate (tag_mask_def |> conv64_RHS |> we_simp |> conv64_RHS |> SIMP_RULE std_ss [shift_left_rwt] |> SIMP_RULE std_ss [Once (GSYM shift_left_rwt),word_2comp_def] |> conv64)
+
+val _ = translate (encode_header_def |> conv64_RHS)
+
+(* Manually inlined: shift_def, bytes_in_word *)
+val inline_simp = SIMP_RULE std_ss [shift_def,bytes_in_word_def]
+
+(* TODO: the wordLang datatype translations run into some weird errors with their no_closures proofs, better investigate that *)
+val _ = translate (StoreEach_def |> inline_simp |> conv64)
+
+val _ = translate (all_ones_def |> conv64_RHS |> we_simp |> SIMP_RULE std_ss [shift_left_rwt,shift_right_rwt] |> wcomp_simp |> conv64 |> wcomp_simp |> conv64)
+
+val _ = translate (maxout_bits_def |> SIMP_RULE std_ss [word_lsl_n2w] |> conv64)
+
+val _ = translate (ptr_bits_def  |> conv64)
+
+val _ = translate (real_addr_def |> inline_simp |> conv64_RHS |> SIMP_RULE std_ss [LET_THM])
+
+val _ = translate (real_offset_def |> inline_simp |> conv64)
+val _ = translate (real_byte_offset_def |> inline_simp |> conv64)
+val _ = translate (GiveUp_def |> wcomp_simp |> conv64)
+
+val _ = matches:= [``foo:'a wordLang$prog``,``foo:'a wordLang$exp``]
+
+val assign_rw = prove(``
+  (i < 0 ⇒ n2w (Num (4 * (0 -i))) = n2w (Num (ABS (4*(0-i))))) ∧
+  (¬(i < 0) ⇒ n2w (Num (4 * i)) = n2w (Num (ABS (4*i))))``,
+  rw[]
+  >-
+    (`0 ≤ 4* -i` by intLib.COOPER_TAC>>
+    fs[GSYM integerTheory.INT_ABS_EQ_ID])
+  >>
+    `0 ≤ 4*i` by intLib.COOPER_TAC>>
+    fs[GSYM integerTheory.INT_ABS_EQ_ID])
+
+(* TODO: word_mul should maybe target a real op ? *)
+
+val _ = translate (assign_def |> SIMP_RULE std_ss [assign_rw] |> inline_simp |> conv64 |> we_simp |> SIMP_RULE std_ss[SHIFT_ZERO,shift_left_rwt] |> SIMP_RULE std_ss [word_mul_def])
+
+val _ = save_thm ("comp_ind",data_to_wordTheory.comp_ind|> conv64|> wcomp_simp)
+val _ = translate (comp_def |> conv64 |> wcomp_simp |> conv64)
+
+val _ = export_theory();
